src/Std/Data/Iterators/Lemmas.lean
@@ -6,7 +6,6 @@ Authors: Paul Reichert
 prelude
 import Init.Data.Iterators.Lemmas.Basic
 import Std.Data.Iterators.Lemmas.Monadic
-import Init.Data.Iterators.Lemmas.Consumers
 import Std.Data.Iterators.Lemmas.Combinators
 import Std.Data.Iterators.Lemmas.Producers
 import Std.Data.Iterators.Lemmas.Equivalence
